CODIGO/SUMA/Auxiliar/Sum.dfy
@@ -65,3 +65,46 @@ lemma GSumIntPartes(A:multiset<int>, P1:multiset<int>, P2:multiset<int>)
     requires P1 <= A && P2 <= A && P1 + P2 == A 
     ensures GSumInt(A) == GSumInt(P1) + GSumInt(P2)
 //Por induccion 
+
+
+method {:verify true} mSumaNat(A:multiset<nat>) returns (s:nat)
+ensures s == GSumNat(A)
+{ var A' := A;
+  s := 0; var e:int; 
+  
+  while |A'| > 0
+  decreases |A'|
+  invariant A' <= A
+  invariant s == GSumNat(A - A')
+   { 
+     e := minInt(A');
+     assert e in A';
+     GSumNatPartes(A - (A'-multiset{e}), A - A',multiset{e});
+     assert s + e == GSumNat(A - (A'-multiset{e}));
+     s := s + e;
+     A' := A' - multiset{e};
+   }
+  assert A' == multiset{} && A - A' == A;
+  assert s == GSumNat(A);
+}
+
+method {:verify true} mSumaInt(A:multiset<int>) returns (s:int)
+ensures s == GSumInt(A)
+{ var A' := A;
+  s := 0; var e:int; 
+  
+  while |A'| > 0
+  decreases |A'|
+  invariant A' <= A
+  invariant s == GSumInt(A - A')
+   { 
+     e := minInt(A');
+     assert e in A';
+     GSumIntPartes(A - (A'-multiset{e}), A - A',multiset{e});
+     assert s + e == GSumInt(A - (A'-multiset{e}));
+     s := s + e;
+     A' := A' - multiset{e};
+   }
+  assert A' == multiset{} && A - A' == A;
+  assert s == GSumInt(A);
+}
