CODIGO/SUMA/Problems/Intervalo.dfy
@@ -9,3 +9,11 @@ ghost predicate Intervalo(A:multiset<nat>, S:nat, T:nat)
 {
   exists I:multiset<nat> | I <= A :: S <= GSumNat(I) < T
 }
+
+method {:verify true} checkIntervalo(A:multiset<nat>, S:nat, T:nat, I:multiset<nat>) returns (b:bool)
+ensures b == (I <= A && S <= GSumNat(I) < T)
+{ 
+  var suma := mSumaNat(I);
+  assert suma == GSumNat(I); 
+  b := I <= A && S <= suma < T; 
+}
