CODIGO/SUMA/Transformations/SumaToIntervalo.dfy
@@ -10,7 +10,7 @@ function Suma_to_Intervalo(A:multiset<nat>, S:nat) : (r:(multiset<nat>, nat, nat
 
 lemma Suma_Intervalo(A:multiset<nat>, S:nat)
   ensures var (IE,IS,IT) := Suma_to_Intervalo(A, S);
-          Suma(A,S) <==> Intervalo(IE,IS,IT)
+          SumaNat(A,S) <==> Intervalo(IE,IS,IT)
 { 
     Suma_Intervalo1(A,S);
     Suma_Intervalo2(A,S);
@@ -18,7 +18,7 @@ lemma Suma_Intervalo(A:multiset<nat>, S:nat)
 
 lemma Suma_Intervalo1(A:multiset<nat>, S:nat)
     ensures var (IE,IS,IT) := Suma_to_Intervalo(A, S);
-          Suma(A,S) <== Intervalo(IE,IS,IT)
+          SumaNat(A,S) <== Intervalo(IE,IS,IT)
 {   
     var (IE,IS,IT) := Suma_to_Intervalo(A,S);
     // IE = {1, 2, 4}, IS = 6, IT = 7
@@ -30,10 +30,10 @@ lemma Suma_Intervalo1(A:multiset<nat>, S:nat)
 
 lemma Suma_Intervalo2(A:multiset<nat>, S:nat)
     ensures var (IE,IS,IT) := Suma_to_Intervalo(A,S);
-          Suma(A,S) ==> Intervalo(IE,IS,IT)
+          SumaNat(A,S) ==> Intervalo(IE,IS,IT)
 {
     // A = {1, 2, 4}, S = 6
-    if (Suma(A,S)) {
+    if (SumaNat(A,S)) {
         var (IE,IS,IT) := Suma_to_Intervalo(A,S);
 
         var C:multiset<int> :| C <= A && GSumNat(C) == S; // C = 2, 4  ->  Sum(C) = 6
